Test/git-issues/git-issue-1604d.dfy
@@ -1,0 +1,59 @@
+// RUN: %dafny /compile:3 /rprint:"%t.rprint" "%s" > "%t"
+// RUN: %diff "%s.expect" "%t"
+
+// Double constraints. Will this still work?
+
+datatype Cell = Cell(x: int)
+
+predicate isNatural(x: int) {
+  x >= 0
+}
+
+// Ghost constraint
+type GhostNaturalCell = c: Cell | isNatural(c.x) witness Cell(0)
+
+// Compilable constraint
+type CompilableNaturalCell = c: GhostNaturalCell | c.x >= 0 witness Cell(0)
+
+
+predicate isNonZero(x: int) {
+  x != 0
+}
+
+// Ghost constraint
+type GhostOrdinalCell = c: GhostNaturalCell | isNonZero(c.x) witness Cell(1)
+// Ghost constraint
+type GhostOrdinalCell2 = c: CompilableNaturalCell | isNonZero(c.x) witness Cell(1)
+// Ghost constraint
+type GhostOrdinalCell3 = c: GhostNaturalCell | c.x != 0 witness Cell(1)
+// Compilable constraint
+type CompilableOrdinalCell = c: CompilableNaturalCell | c.x != 0 witness Cell(1)
+
+predicate method ghostOrdinalCellIsOneOrMore(c: GhostOrdinalCell)
+{
+  (if c.x <= 0 then 1/0 else c.x) > 1
+}
+predicate method compiledOrdinalCellIsOneOrMore(c: CompilableOrdinalCell)
+{
+  (if c.x <= 0 then 1/0 else c.x) > 1
+}
+
+function method returnsOneIfCompilableOrdinalCell(c: CompilableOrdinalCell): int
+{
+  if c.x <= 0 then 1/0 else 1
+}
+function method returnsOneIfGhostOrdinalCell(c: GhostOrdinalCell): int
+{
+  if c.x <= 0 then 1/0 else 1
+}
+
+function method {:opaque} getOriginalSet(): set<Cell> {
+  { Cell(-1), Cell(0), Cell(1), Cell(2) }
+}
+
+predicate method isSetOfGhostOrdinalCells(s: set<GhostOrdinalCell>) {
+  forall c :: c in s ==> returnsOneIfGhostOrdinalCell(c) == 1
+}
+predicate method isSetOfCompilableEvenCells(s: set<CompilableOrdinalCell>) {
+  forall c :: c in s ==> returnsOneIfCompilableOrdinalCell(c) == 1
+}
